src/program_proof/simplepb/pb_start_proof.v
@@ -1,7 +1,7 @@
 From Perennial.program_proof Require Import grove_prelude.
 From Goose.github_com.mit_pdos.gokv.simplepb Require Export pb.
 From Perennial.program_proof.grove_shared Require Import urpc_proof urpc_spec.
-From Perennial.program_proof.simplepb Require Import pb_marshal_proof pb_definitions pb_applybackup_proof pb_setstate_proof pb_getstate_proof pb_becomeprimary_proof pb_apply_proof pb_roapply_proof pb_roapplybackup_proof pb_makeclerk_proof.
+From Perennial.program_proof.simplepb Require Import pb_marshal_proof pb_definitions pb_applybackup_proof pb_setstate_proof pb_getstate_proof pb_becomeprimary_proof pb_apply_proof pb_roapply_proof pb_makeclerk_proof.
 From iris.algebra Require Import mono_list.
 
 Section pb_start_proof.
